experiment/Experiment.Steel.Repr.Test.Extract.fst
@@ -10,9 +10,7 @@ open Steel.Reference
 
 let test3 (r0 r1 : ref U32.t)
   : Steel unit
-      (M.vprop_of_list (Test.test3_mem r0 r1)) (fun x -> M.vprop_of_list (Test.test3_mem r0 r1))
-      (requires fun h0      ->
-        U32.v (M.sel_f (Test.test3_mem r0 r1) h0 0) < 42)
-      (ensures  fun h0 () h1 ->
-        U32.v (M.sel_f (Test.test3_mem r0 r1) h1 1) == U32.v (M.sel_f (Test.test3_mem r0 r1) h0 0) + 1)
-  = Test.test3_steel r0 r1 ()
+      (M.vprop_of_list' (Test.test3_mem r0 r1)) (fun _ -> M.vprop_of_list' (Test.test3_mem r0 r1))
+      (requires fun h0 -> U32.v (sel r0 h0) < 42)
+      (ensures fun h0 () h1 -> U32.v (sel r1 h1) == U32.v (sel r0 h0) + 1)
+  = Test.test3_steel' r0 r1 ()
